Valaig/ForLean.lean
@@ -2,3 +2,4 @@ module
 
 public import Valaig.ForLean.Array
 public import Valaig.ForLean.Iter
+public import Valaig.ForLean.Panic
