Valaig/ForLean/Panic.lean
@@ -1,0 +1,44 @@
+module
+
+public section
+
+@[simp, grind =]
+theorem panic_eq {α : Type} [Inhabited α] {msg : String} :
+    panic (α := α) msg = Inhabited.default := by
+  grind [panic, panicCore]
+
+namespace Valaig
+
+def panicAt {α : Type} [Inhabited α] (loc msg : String) : α :=
+    panic s!"paniced at {loc}: {msg}"
+
+@[simp, grind =]
+theorem panicAt_eq {α : Type} [Inhabited α] {loc msg : String} :
+    panicAt (α := α) loc msg = Inhabited.default := by
+  grind [panicAt]
+
+set_option linter.unusedVariables false in
+@[always_inline]
+def checkOrPanic (p : Prop) [Decidable p] (loc msg : String) : Option { u : Unit // p } :=
+  if h : p then
+    some ⟨(), h⟩
+  else
+    panicAt loc msg
+
+@[simp, grind =]
+theorem checkOrPanic_eq {p : Prop} [Decidable p] {loc msg : String} :
+    checkOrPanic p loc msg = if h : p then some ⟨(), h⟩ else none := by
+  grind [checkOrPanic]
+
+set_option linter.unusedVariables false in
+@[grind .]
+theorem checkOrPanic_some {p : Prop} [Decidable p] {loc msg : String} u
+    (some : checkOrPanic p loc msg = some u) : p := by
+  grind [checkOrPanic]
+
+@[grind .]
+theorem checkOrPanic_none {p : Prop} [Decidable p] {loc msg : String}
+    (none : checkOrPanic p loc msg = none) : ¬p := by
+  grind [checkOrPanic]
+
+end Valaig
